src/extensions/paths/SingletonTyping.v
@@ -1,0 +1,90 @@
+(** printing |-#    %\vdash_{\#}%    #&vdash;<sub>&#35;</sub>#     *)
+(** printing |-##   %\vdash_{\#\#}%  #&vdash;<sub>&#35&#35</sub>#  *)
+(** printing |-##v  %\vdash_{\#\#v}% #&vdash;<sub>&#35&#35v</sub># *)
+(** printing |-!    %\vdash_!%       #&vdash;<sub>!</sub>#         *)
+(** remove printing ~ *)
+
+
+Set Implicit Arguments.
+
+Require Import LibLN.
+Require Import Coq.Program.Equality List.
+Require Import Definitions Binding Narrowing PreciseTyping RecordAndInertTypes
+               Subenvironments TightTyping.
+
+(** * Singleton typing
+
+      Encodes singleton transitivity rule, which we only allow to be obtained directly
+      from the environment. It is like precise typing + following singleton paths *)
+
+Reserved Notation "G '⊢•' p ':' qs '⪼' T" (at level 40, p at level 59).
+
+Inductive ty_path_sngl : ctx -> path -> list path -> typ -> Prop :=
+
+| ty_refl_sngl : forall G p T T',
+    G ⊢! p: T ⪼ T' ->
+    G ⊢• p: nil ⪼ T'
+
+| ty_trans_sngl : forall G p q qs rs T,
+    G ⊢• p: qs ⪼ typ_sngl q ->
+    G ⊢• q: rs ⪼ T ->
+    G ⊢• p: rs ++ (q :: qs) ⪼ T
+
+where "G '⊢•' p ':' qs ⪼ T" := (ty_path_sngl G p qs T).
+
+Hint Constructors ty_path_sngl.
+
+Lemma sngl_bot : forall G p qs,
+    inert G ->
+    G ⊢• p: qs ⪼ typ_bot ->
+    False.
+Proof.
+  introv Hi Hp. dependent induction Hp; eauto. false* pf_bot.
+Qed.
+
+Lemma sngl_and : forall G p qs T U,
+    inert G ->
+    G ⊢• p : qs ⪼ typ_and T U ->
+    G ⊢• p : qs ⪼ T /\ G ⊢• p: qs ⪼ U.
+Proof.
+  introv Hi Hp. dependent induction Hp.
+  - assert (G ⊢! p : T0 ⪼ T /\ G ⊢! p : T0 ⪼ U) as Hpp by constructor*.
+    destruct Hpp as [Hp1 Hp2]; constructor*.
+  - specialize (IHHp2 _ _ Hi eq_refl). destruct IHHp2 as [Hr1 Hr2]. eauto.
+Qed.
+
+Lemma sngl_to_tight: forall G p qs T,
+    G ⊢• p : qs ⪼ T ->
+    G ⊢# trm_path p: T.
+Proof.
+  introv Hp. dependent induction Hp. apply* precise_to_tight. eauto.
+Qed.
+
+Lemma sngl_precise : forall G p q qs T,
+    G ⊢• p : (q :: qs) ⪼ T ->
+    exists U, G ⊢! q: U ⪼ T.
+Proof.
+  introv Hp. dependent induction Hp; eauto.
+  destruct rs.
+  - simpls. inversions x. inversions Hp2. eauto.
+    destruct (app_eq_nil _ _ H). subst. inversion H2.
+  - simpls. inversions x. specialize (IHHp2 _ _ eq_refl). destruct IHHp2 as [U Hp]. eauto.
+Qed.
+
+Lemma sngl_tight_paths : forall G p q qs T,
+    G ⊢• p : (q :: qs) ⪼ T ->
+    G ⊢# trm_path p : typ_sngl q.
+Proof.
+  introv Hp. dependent induction Hp; eauto.
+  destruct rs; simpls; inversions x. apply* sngl_to_tight.
+  specialize (IHHp2 _ _ eq_refl). apply sngl_to_tight in Hp1. apply ty_sub_t with (T:=typ_sngl q0); auto.
+  assert (typ_sngl q = repl_typ q0 q (typ_sngl q0)) as Heq by admit. rewrite* Heq.
+Qed.
+
+Lemma sngl_inertsngl : forall G p qs T,
+    inert G ->
+    G ⊢• p: qs ⪼ T ->
+    inert_sngl T \/ record_type T.
+Proof.
+  introv Hi Hp. induction Hp; eauto. apply* pf_inertsngl.
+Qed.
